src/note.lean
@@ -1,0 +1,3 @@
+set_option pp.all true
+constant x : ℕ → Prop
+#check ∃ p,x p
