src/ntac/semantic_tree.lean
@@ -9,7 +9,7 @@ meta inductive semantic_tree : Type
 | have_exact : expr → semantic_tree → semantic_tree
 | have_from : semantic_tree → semantic_tree → semantic_tree
 | let_from : semantic_tree → semantic_tree → semantic_tree
-| have_triv : expr → semantic_tree
+| have_triv : expr → semantic_tree → semantic_tree
 | suffice_from : expr → semantic_tree → semantic_tree → semantic_tree
 | exact : expr → semantic_tree
 | trivial : semantic_tree
@@ -19,12 +19,14 @@ meta inductive semantic_tree : Type
 
 meta def tolistS : semantic_tree → list S :=
 λ s,match s with
+| semantic_tree.unresolved := [S._unresolved]
 | semantic_tree.trivial := [S._trivial]
 | semantic_tree.init s := tolistS s
 | semantic_tree.suffice_from e t1 t2 :=tolistS t1 ++ Adv._hence /a/ <eNP>e /p/ <VVP>V._suf_show :: tolistS t2
 | semantic_tree.have_from t1 t2 := tolistS t1 ++ tolistS t2
+| semantic_tree.have_triv e t2 := Adv._trivially /a/ <eS>e :: tolistS t2
 | semantic_tree.assume_prop e t:= /i/ <V2VP>V2._assume <eNP>e :: tolistS t
-| semantic_tree.exact e := [Adv._from_assum /a/ <S>e]
+| semantic_tree.exact e := [Adv._from_assum /a/ <eS>e]
 | semantic_tree.assume_val edef eval t:= /i/ <V3VP> V3._let <NP><eN>edef <NP><eN>eval :: tolistS t
 | semantic_tree.assume_exist e t := [S._trivial]
 | semantic_tree.have_exact e t := Adv._from <NP><eN>e /a/ S._trivial :: tolistS t
